Restore the previous aps_plus definition. It cannot be verified using the current framework but neither can the last one because of function calls (take for instance the APS transformation of [loop () + ()]). Conclusion: either modify the semantics to do some dynamic checks after evaluating each side of a binary operation or introduce typing (that would imply that the evaluation of each side of a binary operation may only yield an integer).

theories/aps_plus/examples/list_length.v
@@ -38,49 +38,35 @@ Definition list_length_aps_plus : data_human_program := {[
       NIL =>
         0 + "acc"
     | CONS "<>", "xs" =>
-        let: "acc'" := 1 in
+        let: "acc" := 1 + "acc" in
         let: "arg" := "xs" in
-        $"list_length_aps" ("acc'" + "acc", "arg")
+        $"list_length_aps" ("acc", "arg")
     end
   )%data_human_expr)
 ]}.
 
-Goal
-  aps_plus
-    (data_human_program_compile list_length)
-    (data_human_program_compile list_length_aps_plus).
-Proof.
-  rewrite /list_length /list_length_aps_plus.
-  rewrite /data_human_program_compile map_fmap_singleton fmap_insert map_fmap_singleton /=.
-  exists {["list_length" := "list_length_aps"]}; try set_solver.
-  + intros * (<- & <-)%lookup_singleton_Some.
-    rewrite lookup_insert.
-    eexists. split; last done. repeat econstructor.
-  + intros * (<- & <-)%lookup_singleton_Some (_ & <-)%lookup_singleton_Some.
-    eexists. split; last done.
-    repeat constructor. eapply aps_plus_aps_plus_1; first constructor.
-    * eapply aps_plus_aps_call; repeat constructor.
-    * done.
-Qed.
+Section list_length_aps_plus_sound.
+  Variable aps_plus_sound : ∀ progₛ progₜ,
+    data_program_valid progₛ →
+    aps_plus progₛ progₜ →
+    data_program_refinement progₛ progₜ.
 
-(* Lemma list_length_aps_plus_sound : *)
-(*   data_program_refinement *)
-(*     (data_human_program_compile list_length) *)
-(*     (data_human_program_compile list_length_aps_plus). *)
-(* Proof. *)
-(*   rewrite /list_length /list_length_aps_plus. apply aps_plus_sound. *)
-(*   - split. *)
-(*     + apply data_human_program_compile_well_formed. *)
-(*       rewrite /data_human_program_well_formed map_Forall_singleton //. *)
-(*     + apply data_human_program_compile_scope. *)
-(*   - rewrite /data_human_program_compile map_fmap_singleton fmap_insert map_fmap_singleton /=. *)
-(*     exists {["list_length" := "list_length_aps"]}; try set_solver. *)
-(*     + intros * (<- & <-)%lookup_singleton_Some. *)
-(*       rewrite lookup_insert. *)
-(*       eexists. split; last done. repeat econstructor. *)
-(*     + intros * (<- & <-)%lookup_singleton_Some (_ & <-)%lookup_singleton_Some. *)
-(*       eexists. split; last done. *)
-(*       repeat constructor. eapply aps_plus_aps_plus_1; first constructor. *)
-(*       * eapply aps_plus_aps_call; repeat constructor. *)
-(*       * done. *)
-(* Qed. *)
+  Lemma list_length_aps_plus_sound :
+    data_program_refinement
+      (data_human_program_compile list_length)
+      (data_human_program_compile list_length_aps_plus).
+  Proof using aps_plus_sound.
+    rewrite /list_length /list_length_aps_plus. apply aps_plus_sound.
+    - split.
+      + apply data_human_program_compile_well_formed.
+        rewrite /data_human_program_well_formed map_Forall_singleton //.
+      + apply data_human_program_compile_scope.
+    - rewrite /data_human_program_compile map_fmap_singleton fmap_insert map_fmap_singleton /=.
+      exists {["list_length" := "list_length_aps"]}; try set_solver.
+      + intros * (<- & <-)%lookup_singleton_Some.
+        rewrite lookup_insert.
+        eexists. split; last done. repeat econstructor.
+      + intros * (<- & <-)%lookup_singleton_Some (_ & <-)%lookup_singleton_Some.
+        eexists. split; last done. repeat econstructor.
+  Qed.
+End list_length_aps_plus_sound.
